Makefile
@@ -311,7 +311,7 @@ HMAC_FILES= \
   verif_hmac_double.v verif_hmac_crypto.v protocol_spec_hmac.v
 
 HKDF_FILES= \
-  hkdf_functional_prog.v hkdf.v hkdf_compspecs.v spec_hkdf.v \
+  hkdf_functional_prog.v hkdf.v spec_hkdf.v \
   verif_hkdf_extract.v verif_hkdf_expand.v verif_hkdf.v
 
 FCF_FILES= \
